after synchron

Environment.v
@@ -142,6 +142,105 @@ Section Global.
       + right; auto.
   Qed.
 
+  Definition adds xs (vs : list A) (e : t A) :=
+    fold_right (fun (xv: ident * A) env =>
+                  let (x , v) := xv in
+                  add x v env) e (combine xs vs).
+
+  Lemma add_comm:
+    forall x x' (v v': A) m,
+      x <> x' ->
+      add x v (add x' v' m) = add x' v' (add x v m).
+  Proof.
+    Ltac aux :=
+      try match goal with
+          (* | H: POTB.lt ?x' ?y, H': POTB.lt ?y ?x, H'': POTB.lt ?x ?x' |- _ => *)
+          (*   let E := fresh in *)
+          (*   assert (POTB.lt x' x) by (now transitivity y); *)
+          (*   assert (POTB.lt x' x') as E by (now transitivity x); *)
+          (*   apply POTB.lt_not_eq in E; exfalso; apply E; reflexivity *)
+          | H: POTB.lt ?x ?x', H': POTB.eq ?x' ?x |- _ =>
+            apply POTB.lt_not_eq in H; symmetry in H'; contradiction
+          | H: POTB.lt ?x ?x', H': POTB.eq ?x ?x' |- _ =>
+            apply POTB.lt_not_eq in H; contradiction
+          | H: POTB.lt ?x ?x', H': POTB.lt ?x' ?x |- _ =>
+            let E := fresh in
+            assert (POTB.lt x x) as E by (now transitivity x');
+            apply POTB.lt_not_eq in E; exfalso; apply E; reflexivity
+          | H: POTB.lt ?x ?x', H': POTB.lt ?x' ?y, H'': POTB.eq ?x ?y |- _ =>
+            let E := fresh in
+            assert (POTB.lt x y) as E by (now transitivity x');
+            apply POTB.lt_not_eq in E; contradiction
+          | H: POTB.lt ?x ?x', H': POTB.lt ?x' ?y, H'': POTB.eq ?y ?x |- _ =>
+            let E := fresh in
+            assert (POTB.lt x y) as E by (now transitivity x');
+            apply POTB.lt_not_eq in E; symmetry in H''; contradiction
+          | H: ?x <> ?x', H': POTB.eq ?x' ?y, H'': POTB.eq ?x ?y |- _ =>
+            exfalso; apply H; now rewrite H', H''
+          | H: ?x <> ?x', H': POTB.eq ?x' ?x |- _ =>
+            exfalso; apply H; now rewrite H'
+          | H: POTB.eq ?x' ?y, H': POTB.lt ?y ?x, H'': POTB.lt ?x ?x' |- _ =>
+            rewrite H in H'';
+            let E := fresh in
+            assert (POTB.lt x x) as E by (now transitivity y);
+            apply POTB.lt_not_eq in E; exfalso; apply E; reflexivity
+           end; try contradiction; auto.
+
+    intros ** Neq.
+    revert dependent x; revert v v' x'; induction m as [|(y, w)]; simpl; intros.
+    - destruct (POTB.compare x x'), (POTB.compare x' x); aux.
+    - destruct (POTB.compare x' y) eqn: E, (POTB.compare x y) eqn: E'; simpl;
+        try rewrite E; try rewrite E'; try (f_equal; auto);
+          try destruct (POTB.compare x x'); try destruct (POTB.compare x' x); aux.
+      + assert (POTB.lt x' x) by (now transitivity y);
+          assert (POTB.lt x' x') as E'' by (now transitivity x);
+          apply POTB.lt_not_eq in E''; exfalso; apply E''; reflexivity.
+      + assert (POTB.lt y x) by (now transitivity x');
+          assert (POTB.lt y y) as E'' by (now transitivity x);
+          apply POTB.lt_not_eq in E''; exfalso; apply E''; reflexivity.
+  Qed.
+
+  Lemma adds_cons_cons:
+    forall xs x (v: A) vs e,
+      ~ In x xs ->
+      adds (x :: xs) (v :: vs) e = adds xs vs (add x v e).
+  Proof.
+    unfold adds.
+    induction xs as [|x']; intros ** NotIn; simpl; auto.
+    destruct vs as [|v']; simpl; auto.
+    rewrite <-IHxs.
+    - simpl.
+      rewrite add_comm; auto.
+      intro Eq.
+      apply NotIn; subst.
+      apply in_eq.
+    - now apply not_in_cons in NotIn.
+  Qed.
+
+  Lemma find_gsso:
+    forall x x' xs (vs: list A) S,
+      x <> x' ->
+      find x (adds (x' :: xs) vs S) = find x (adds xs (tl vs) S).
+  Proof.
+    intros ** Hneq.
+    unfold adds.
+    destruct vs. destruct xs; reflexivity.
+    simpl. rewrite gso; auto.
+  Qed.
+
+  Lemma NotInMembers_find_adds:
+    forall x xs (v: option A) vs S,
+      ~In x xs ->
+      find x S = v ->
+      find x (adds xs vs S) = v.
+  Proof.
+    induction xs as [|xty xs]; auto.
+    intros v vs S Hnin Hfind.
+    apply not_in_cons in Hnin.
+    destruct Hnin as [Hnin Hneq].
+    rewrite find_gsso; auto.
+  Qed.
+
 End Global.
 
 Theorem find_map:
