NLustre.v
@@ -1,11 +1,13 @@
 Require Import Operators.
 Require Import Clocks.
 Require Export NLustre.Stream.
+Require Import NLustre.NLExprSyntax.
 Require Export NLustre.NLSyntax.
 Require Export NLustre.IsFree.
 Require Export NLustre.IsVariable.
 Require Export NLustre.IsDefined.
 Require Export NLustre.Memories.
+Require Import NLustre.NLExprSemantics.
 Require Export NLustre.NLSemantics.
 Require Export NLustre.MemSemantics.
 Require Export NLustre.WellFormed.
@@ -22,21 +24,23 @@ Module Type NLUSTRE
        (Op    : OPERATORS)
        (OpAux : OPERATORS_AUX Op)
        (Clks  : CLOCKS Ids).
-  Declare Module Export Syn: NLSYNTAX        Ids Op       Clks.
-  Declare Module Export Str: STREAM              Op OpAux.
-  Declare Module Export Ord: ORDERED         Ids Op       Clks Syn.
-  Declare Module Export IsF: ISFREE          Ids Op       Clks Syn.
-  Declare Module Export Sem: NLSEMANTICS     Ids Op OpAux Clks Syn Str Ord.
-  Declare Module Export Typ: NLTYPING        Ids Op       Clks Syn.
-  Declare Module Export Mem: MEMORIES        Ids Op       Clks Syn.
-  Declare Module Export IsD: ISDEFINED       Ids Op       Clks Syn             Mem.
-  Declare Module Export IsV: ISVARIABLE      Ids Op       Clks Syn             Mem IsD.
-  Declare Module Export NoD: NODUP           Ids Op       Clks Syn             Mem IsD IsV.
-  Declare Module Export WeF: WELLFORMED      Ids Op       Clks Syn     Ord     Mem IsD IsV IsF NoD.
-  Declare Module Export MemSem: MEMSEMANTICS Ids Op OpAux Clks Syn Str Ord Sem Mem IsD IsV IsF NoD WeF.
-  Declare Module Export Clo: NLCLOCKING      Ids Op       Clks Syn             Mem IsD     IsF.
+  Declare Module Export ExprSyn: NLEXPRSYNTAX        Op.
+  Declare Module Export Syn    : NLSYNTAX        Ids Op       Clks ExprSyn.
+  Declare Module Export Str    : STREAM              Op OpAux.
+  Declare Module Export Ord    : ORDERED         Ids Op       Clks ExprSyn Syn.
+  Declare Module Export IsF    : ISFREE          Ids Op       Clks ExprSyn Syn.
+  Declare Module Export ExprSem: NLEXPRSEMANTICS Ids Op OpAux Clks ExprSyn     Str.
+  Declare Module Export Sem    : NLSEMANTICS     Ids Op OpAux Clks ExprSyn Syn Str Ord ExprSem.
+  Declare Module Export Typ    : NLTYPING        Ids Op       Clks ExprSyn Syn.
+  Declare Module Export Mem    : MEMORIES        Ids Op       Clks ExprSyn Syn.
+  Declare Module Export IsD    : ISDEFINED       Ids Op       Clks ExprSyn Syn                     Mem.
+  Declare Module Export IsV    : ISVARIABLE      Ids Op       Clks ExprSyn Syn                     Mem IsD.
+  Declare Module Export NoD    : NODUP           Ids Op       Clks ExprSyn Syn                     Mem IsD IsV.
+  Declare Module Export WeF    : WELLFORMED      Ids Op       Clks ExprSyn Syn     Ord             Mem IsD IsV IsF NoD.
+  Declare Module Export MemSem : MEMSEMANTICS    Ids Op OpAux Clks ExprSyn Syn Str Ord ExprSem Sem Mem IsD IsV IsF NoD WeF.
+  Declare Module Export Clo    : NLCLOCKING      Ids Op       Clks ExprSyn Syn                     Mem IsD     IsF.
 
-  Declare Module Scheduler: NLSCHEDULE       Ids Op OpAux Clks Syn Str Ord Sem Mem IsD     IsF          Typ Clo.
+  Declare Module Scheduler     : NLSCHEDULE      Ids Op OpAux Clks ExprSyn Syn Str Ord ExprSem Sem Mem IsD     IsF          Typ Clo.
 
 End NLUSTRE.
 
@@ -46,20 +50,22 @@ Module NLustreFun
        (OpAux : OPERATORS_AUX Op)
        (Clks  : CLOCKS Ids)
        <: NLUSTRE Ids Op OpAux Clks.
-  Module Export Syn := NLSyntaxFun        Ids Op       Clks.
-  Module Export Str := StreamFun              Op OpAux.
-  Module Export Ord := OrderedFun         Ids Op       Clks Syn.
-  Module Export IsF := IsFreeFun          Ids Op       Clks Syn.
-  Module Export Sem := NLSemanticsFun     Ids Op OpAux Clks Syn Str Ord.
-  Module Export Typ := NLTypingFun        Ids Op       Clks Syn.
-  Module Export Mem := MemoriesFun        Ids Op       Clks Syn.
-  Module Export IsD := IsDefinedFun       Ids Op       Clks Syn             Mem.
-  Module Export IsV := IsVariableFun      Ids Op       Clks Syn             Mem IsD.
-  Module Export NoD := NoDupFun           Ids Op       Clks Syn             Mem IsD IsV.
-  Module Export WeF := WellFormedFun      Ids Op       Clks Syn     Ord     Mem IsD IsV IsF NoD.
-  Module Export MemSem := MemSemanticsFun Ids Op OpAux Clks Syn Str Ord Sem Mem IsD IsV IsF NoD WeF.
-  Module Export Clo := NLClockingFun      Ids Op       Clks Syn             Mem IsD     IsF.
+  Module Export ExprSyn := NLExprSyntaxFun        Op.
+  Module Export Syn     := NLSyntaxFun        Ids Op       Clks ExprSyn.
+  Module Export Str     := StreamFun              Op OpAux.
+  Module Export Ord     := OrderedFun         Ids Op       Clks ExprSyn Syn.
+  Module Export IsF     := IsFreeFun          Ids Op       Clks ExprSyn Syn.
+  Module Export ExprSem := NLExprSemanticsFun Ids Op OpAux Clks ExprSyn     Str.
+  Module Export Sem     := NLSemanticsFun     Ids Op OpAux Clks ExprSyn Syn Str Ord ExprSem.
+  Module Export Typ     := NLTypingFun        Ids Op       Clks ExprSyn Syn.
+  Module Export Mem     := MemoriesFun        Ids Op       Clks ExprSyn Syn.
+  Module Export IsD     := IsDefinedFun       Ids Op       Clks ExprSyn Syn                     Mem.
+  Module Export IsV     := IsVariableFun      Ids Op       Clks ExprSyn Syn                     Mem IsD.
+  Module Export NoD     := NoDupFun           Ids Op       Clks ExprSyn Syn                     Mem IsD IsV.
+  Module Export WeF     := WellFormedFun      Ids Op       Clks ExprSyn Syn     Ord             Mem IsD IsV IsF NoD.
+  Module Export MemSem  := MemSemanticsFun    Ids Op OpAux Clks ExprSyn Syn Str Ord ExprSem Sem Mem IsD IsV IsF NoD WeF.
+  Module Export Clo     := NLClockingFun      Ids Op       Clks ExprSyn Syn                     Mem IsD     IsF.
 
-  Module Scheduler := NLScheduleFun       Ids Op OpAux Clks Syn Str Ord Sem Mem IsD IsF              Typ Clo.
+  Module Scheduler      := NLScheduleFun      Ids Op OpAux Clks ExprSyn Syn Str Ord ExprSem Sem Mem IsD IsF              Typ Clo.
 
 End NLustreFun.
